secure_api/box/Box.ODH.fst
@@ -16,69 +16,56 @@ let rec random_bytes n =
   | 0 -> let l:lbytes 0 = createL [] in l
   | _ -> append (createL [0x0buy]) (random_bytes (n-1))
 
-let sh_hon #oparams sh = sh.h
-
-let exp_hon #oparams exp = exp.sh.h
-
 let get_exp_share #oparams e = e.sh
 
 let get_share_raw #oparams sh = sh.raw_sh
 
 let get_exponent_raw #oparams exp = exp.raw_exp
 
-let gen_dh (oparam:odh_parameters) =
+let gen_dh #rgn ip oparam =
   let raw_exp = random_bytes oparam.exponent_length in
   let raw_sh = oparam.exponentiate raw_exp oparam.generator in
-  let sh = SH raw_sh true in
-  EXP raw_exp sh
+  let h0 = get() in
+  assume(fresh ip (PK_id raw_sh) h0);
+  register ip (PK_id raw_sh) true;
+  let sh = SH raw_sh in
+  (EXP raw_exp sh,sh)
 
-let coerce_dh_sh  (oparam:odh_parameters) (raw_sh:lbytes oparam.share_length) =
-  SH raw_sh false
+let coerce_dh_sh #rgn ip oparam raw_sh =
+  register ip (PK_id raw_sh) false;
+  SH raw_sh
 
-let coerce_dh_exp  (oparam:odh_parameters) (raw_exp:lbytes oparam.exponent_length) =
+let coerce_dh_exp #rgn ip oparam raw_exp =
   let raw_sh = oparam.exponentiate raw_exp oparam.generator in
-  let sh = SH raw_sh false in
+  register ip (PK_id raw_sh) false;
+  let sh = SH raw_sh in
   EXP raw_exp sh
 
-let create_id #oparam sh1 sh2 =
-  let int_sh1 = little_endian sh1.raw_sh in
-  let int_sh2 = little_endian sh2.raw_sh in
-  //let int_sh1 = int_of_bytes sh1.raw_sh in
-  //let int_sh2 = int_of_bytes sh2.raw_sh in
-  if int_sh1 < int_sh2 then
-    (sh1.raw_sh,sh2.raw_sh)
-  else
-    (sh2.raw_sh,sh1.raw_sh)
+let get_op_rgn #rgn #ip #key_length #key_type #kp #oparam op = op.kp_log_rgn
 
-let lemma_symmetric_id #oparam sh1 sh2 =
-  lemma_little_endian_bij sh1.raw_sh sh2.raw_sh
+let get_op_log #rgn #ip #key_length #key_type #kp #oparam op = op.kp_log
 
-let get_flag #key_length #key_type #kp #oparam op = op.b
-
-let get_op_rgn (#key_length:(n:nat{n<=32})) (#key_type:(id -> Type0)) (#kp:key_package key_length key_type) (#oparam:odh_parameters{oparam.hash_length = key_length}) (op:odh_package #key_length #key_type kp oparam) = op.rgn
-
-let get_op_log (#key_length:(n:nat{n<=32})) (#key_type:(id -> Type0)) (#kp:key_package key_length key_type) (#oparam:odh_parameters{oparam.hash_length = key_length}) (op:odh_package #key_length #key_type kp oparam) = op.kp_log
-
-let recall_op_log #key_length #key_type #kp #oparam op =
+let recall_op_log #rgn #ip #key_length #key_type #kp #oparam op =
   recall op.kp_log
 
-let create_odh_package (#key_length:(n:nat{n<=32})) (#key_type:(id -> Type0)) (kp:key_package key_length key_type) (oparam:odh_parameters{oparam.hash_length = key_length}) (rgn:erid) (b:bool) =
+let create_odh_package #rgn #ip #key_length #key_type kp oparam =
   let odh_rgn = new_region rgn in
   let kp_log = MM.alloc #odh_rgn #key_package_log_key #(key_package_log_range key_type) #(key_package_log_inv key_type) in
-  ODH odh_rgn b kp_log
+  ODH odh_rgn kp_log
 
 #set-options "--z3rlimit 300 --max_ifuel 2 --max_fuel 1"
-let dh_op #key_length #key_type #kp #oparam op sh exp =
-  let both_honest = sh.h && exp.sh.h in
-  let i = create_id sh exp.sh in
-    if op.b && both_honest then
+let dh_op #rgn #ip #key_length #key_type #kp #oparam op sh exp =
+  let i = compose_id (PK_id sh.raw_sh) (PK_id exp.sh.raw_sh) in
+  let both_honest = get_honesty ip i in
+    if Flags.prf_odh && both_honest then
       (recall op.kp_log;
       match MM.lookup op.kp_log i with
       | None ->
-        let k:(k:key_type i{kp.hon k = true}) = kp.gen i in
+        //let k:(k:key_type i{kp.hon k = true}) = kp.gen i in
+        let k = kp.gen i in
         MM.extend op.kp_log i k;
         k
       | Some k -> k)
     else
       (recall op.kp_log;
-      kp.cset i (oparam.hash (oparam.exponentiate exp.raw_exp sh.raw_sh)))
+      kp.coerce i (oparam.hash (oparam.exponentiate exp.raw_exp sh.raw_sh)))
