secure_api/box/Box.PKAE.fst
@@ -9,28 +9,30 @@ open FStar.Endianness
 
 open Box.Plain
 
-//module AE = Box.AE
-//module ODH = Box.ODH
-//module MM = FStar.Monotonic.Map
-//module AE_Spec = Spec.SecretBox
-//module ODH_Spec = Spec.Curve25519
-//module H = Spec.HSalsa20
-//
-//assume val random_bytes: n:(n:nat{n<=32}) -> unit -> lbytes n
+module AE = Box.AE
+module ODH = Box.ODH
+module MM = FStar.Monotonic.Map
+module AE_Spec = Spec.SecretBox
+module ODH_Spec = Spec.Curve25519
+module H = Spec.HSalsa20
+
+assume val random_bytes: n:nat -> lbytes n
 //
 //assume val pkae_flag: bool
-//
-//#set-options "--z3rlimit 300 --max_ifuel 1 --max_fuel 1"
-//// For some reason it doesn't verify if there is an additional refinement on the output of secretbox_open_easy
-//let secretbox_scheme =
-//  AE.ES #(AE_Spec.keylen) #(AE_Spec.noncelen) (fun n -> n / Spec.Salsa20.blocklen < pow2 32) (fun n -> n >= 16 && (n - 16) / Spec.Salsa20.blocklen < pow2 32) (random_bytes 32) AE_Spec.secretbox_easy AE_Spec.secretbox_open_easy
-//
-//let ae_params = AE.GP AE_Spec.keylen AE_Spec.noncelen secretbox_scheme
-//
-//let pp = PP (AE.get_ae_flagGT ae_params) (fun n -> n / Spec.Salsa20.blocklen < pow2 32)
-//
-//let kp = AE.create_ae_key_package ODH.id AE_Spec.keylen
-//
+
+val enc_star: n:(n:nat{AE_Spec.valid_plain_length n}) -> b:lbytes (n+16){AE_Spec.valid_cipher_length (n+16)}
+let enc_star n = Seq.append (random_bytes n) (random_bytes 16)
+
+#set-options "--z3rlimit 300 --max_ifuel 2 --max_fuel 2"
+// For some reason it doesn't verify if there is an additional refinement on the output of secretbox_open_easy
+let secretbox_scheme =
+  AE.ES #(AE_Spec.keylen) #(AE_Spec.noncelen) (AE_Spec.valid_plain_length) (AE_Spec.valid_cipher_length) (fun () -> random_bytes 32) AE_Spec.secretbox_easy (enc_star) AE_Spec.secretbox_open_easy
+
+let ae_params = AE.GP AE_Spec.keylen AE_Spec.noncelen secretbox_scheme
+
+let pp = PP (Flags.pkae) (fun n -> n / Spec.Salsa20.blocklen < pow2 32)
+
+
 //let ae_package_log_key = i:ODH.id
 //let ae_package_log_value (rgn:erid) (i:ODH.id) = (ap:AE.ae_package #ODH.id #i #AE_Spec.keylen kp ae_params pp{extends (AE.get_ap_rgn ap) rgn})
 //let ae_package_log_range (rgn:erid) (k:ae_package_log_key) = ae_package_log_value rgn k
@@ -38,222 +40,224 @@ open Box.Plain
 //
 //let ae_package_log (log_rgn:erid) (ap_rgn:erid) =
 //  MM.t log_rgn (ae_package_log_key) (ae_package_log_range ap_rgn) (ae_package_log_inv ap_rgn)
-//
-//let zero_nonce = Seq.create H.noncelen (UInt8.uint_to_t 0)
-//let hsalsa20_hash input = H.hsalsa20 input zero_nonce
-//
-//let odh_params = ODH.OP (ODH_Spec.serialized_point_length) (ODH_Spec.scalar_length) (H.keylen) (ODH_Spec.base_point) (ODH_Spec.scalarmult) (hsalsa20_hash)
-//
-//noeq abstract type pkae_package =
-//  | PKAE_P :
-//    op_rgn:erid ->
-//    op: ODH.odh_package #AE_Spec.keylen #(AE.key AE_Spec.keylen #ODH.id) kp odh_params{extends (ODH.get_op_rgn op) op_rgn} ->
-//    ap_log_rgn:erid{disjoint op_rgn ap_log_rgn} ->
-//    ap_rgn:erid{disjoint op_rgn ap_rgn /\ disjoint ap_rgn ap_log_rgn /\ disjoint (ODH.get_op_rgn op) ap_rgn} ->
-//    ap_log: ae_package_log ap_log_rgn ap_rgn ->
-//    pkae_package
-//
-//val create_pkae_package: rgn:erid -> ST pkae_package
-//  (requires (fun h0 -> True))
-//  (ensures (fun h0 pkae_p h1 ->
-//    modifies (Set.singleton rgn) h0 h1
+
+let zero_nonce = Seq.create H.noncelen (UInt8.uint_to_t 0)
+let hsalsa20_hash input = H.hsalsa20 input zero_nonce
+
+let odh_params = ODH.OP (ODH_Spec.serialized_point_length) (ODH_Spec.scalar_length) (H.keylen) (ODH_Spec.base_point) (ODH_Spec.scalarmult) (hsalsa20_hash)
+
+
+noeq abstract type pkae_package (rgn:erid) =
+  | PKAE_P :
+    pkae_rgn:erid{extends pkae_rgn rgn} ->
+    ip: index_package pkae_rgn ->
+    kp: Key.key_package ip AE_Spec.keylen (AE.key AE_Spec.keylen) ->
+    op: ODH.odh_package #pkae_rgn #ip #AE_Spec.keylen #(AE.key AE_Spec.keylen) kp odh_params ->
+    pkae_package rgn
+
+let ip = create_index_package
+
+val create_pkae_package: rgn:erid -> ST pkae_package
+  (requires (fun h0 -> True))
+  (ensures (fun h0 pkae_p h1 ->
+    modifies (Set.singleton rgn) h0 h1
+    /\ extends (ODH.get_op_rgn pkae_p.op) pkae_p.op_rgn
+  ))
+let create_pkae_package rgn =
+  let pkae_rgn = new_region rgn in
+  let odh_rgn = new_region pkae_rgn in
+  let op = ODH.create_odh_package kp odh_params odh_rgn in
+  let ap_log_rgn = new_region pkae_rgn in
+  let ap_rgn = new_region pkae_rgn in
+  let ap_log = MM.alloc #ap_log_rgn #ae_package_log_key #(ae_package_log_range ap_rgn) #(ae_package_log_inv ap_rgn) in
+  PKAE_P odh_rgn op ap_log_rgn ap_rgn ap_log
+
+let pkey = ODH.share odh_params
+let skey = ODH.exponent odh_params
+let nonce = AE.nonce ae_params
+let ciphertext = AE.ciphertext ae_params
+let gen = ODH.gen_dh odh_params
+
+#set-options "--z3rlimit 300 --max_ifuel 0 --max_fuel 0"
+val get_ap_from_log: pkae_p:pkae_package -> i:ODH.id -> ST (option (ap:ae_package_log_value pkae_p.ap_rgn i))
+  (requires (fun h0 -> True))
+  (ensures (fun h0 ap h1 ->
+    (match sel h0 pkae_p.ap_log i with
+      | Some ap ->
+        contains h1 (AE.get_ap_log ap)
+        /\ MM.defined pkae_p.ap_log i h1
+        /\ MM.contains pkae_p.ap_log i ap h1
+        /\ witnessed (MM.defined pkae_p.ap_log i)
+        /\ witnessed (MM.contains pkae_p.ap_log i ap)
+      | None -> MM.fresh pkae_p.ap_log i h1)
+    /\ h0 == h1
+    /\ ap == MM.sel (sel h1 pkae_p.ap_log) i
+  ))
+
+let get_ap_from_log pkae_p i =
+  match MM.lookup pkae_p.ap_log i with
+  | Some ap ->
+    AE.recall_log ap;
+    Some ap
+  | None -> None
+
+
+//#set-options "--z3rlimit 300 --max_ifuel 0 --max_fuel 0"
+//val nonce_freshness_framing_lemma: pkae_p:pkae_package -> i:ODH.id -> n:nonce -> h0:mem -> h1:mem -> Lemma
+//  (requires (
+//    //((modifies (Set.singleton (ODH.get_op_rgn pkae_p.op)) h0 h1 /\ (extends (ODH.get_op_rgn pkae_p.op) pkae_p.op_rgn)) \/ h0 == h1)
+//    (modifies (Set.singleton (ODH.get_op_rgn pkae_p.op)) h0 h1 \/ h0 == h1)
 //    /\ extends (ODH.get_op_rgn pkae_p.op) pkae_p.op_rgn
+//    /\ disjoint (ODH.get_op_rgn pkae_p.op) pkae_p.ap_log_rgn
+//    /\ contains h0 pkae_p.ap_log
+//    /\ (match sel h0 pkae_p.ap_log i with
+//      | Some ap -> contains h0 (AE.get_ap_log ap)
+//      | None -> True)
 //  ))
-//let create_pkae_package rgn =
-//  let pkae_rgn = new_region rgn in
-//  let odh_rgn = new_region pkae_rgn in
-//  let op = ODH.create_odh_package kp odh_params odh_rgn in
-//  let ap_log_rgn = new_region pkae_rgn in
-//  let ap_rgn = new_region pkae_rgn in
-//  let ap_log = MM.alloc #ap_log_rgn #ae_package_log_key #(ae_package_log_range ap_rgn) #(ae_package_log_inv ap_rgn) in
-//  PKAE_P odh_rgn op ap_log_rgn ap_rgn ap_log
-//
-//let pkey = ODH.share odh_params
-//let skey = ODH.exponent odh_params
-//let nonce = AE.nonce ae_params
-//let ciphertext = AE.ciphertext ae_params
-//let gen = ODH.gen_dh odh_params
-//
-//#set-options "--z3rlimit 300 --max_ifuel 0 --max_fuel 0"
-//val get_ap_from_log: pkae_p:pkae_package -> i:ODH.id -> ST (option (ap:ae_package_log_value pkae_p.ap_rgn i))
-//  (requires (fun h0 -> True))
-//  (ensures (fun h0 ap h1 ->
-//    (match sel h0 pkae_p.ap_log i with
-//      | Some ap ->
-//        contains h1 (AE.get_ap_log ap)
-//        /\ MM.defined pkae_p.ap_log i h1
-//        /\ MM.contains pkae_p.ap_log i ap h1
-//        /\ witnessed (MM.defined pkae_p.ap_log i)
-//        /\ witnessed (MM.contains pkae_p.ap_log i ap)
-//      | None -> MM.fresh pkae_p.ap_log i h1)
-//    /\ h0 == h1
-//    /\ ap == MM.sel (sel h1 pkae_p.ap_log) i
+//  (ensures (
+//    contains h1 pkae_p.ap_log
+//    /\ (match sel h0 pkae_p.ap_log i with
+//      | Some ap_old ->
+//        let ap_new = Some?.v (sel h1 pkae_p.ap_log i) in
+//        AE.get_ap_log ap_old == AE.get_ap_log ap_new
+//        /\ contains h1 (AE.get_ap_log ap_new)
+//      | None -> True)
+//    ///\ (let ap_option_new = sel h1 pkae_p.ap_log i in
+//    //ap_option_new == ap_option_old
+//    ///\ (Some? ap_option_new)
+//    ///\ AE.get_ap_log (Some?.v ap_option_new) == AE.get_ap_log (Some?.v ap_option_old))
 //  ))
-//
-//let get_ap_from_log pkae_p i =
-//  match MM.lookup pkae_p.ap_log i with
-//  | Some ap ->
-//    AE.recall_log ap;
-//    Some ap
-//  | None -> None
-//
-//
-////#set-options "--z3rlimit 300 --max_ifuel 0 --max_fuel 0"
-////val nonce_freshness_framing_lemma: pkae_p:pkae_package -> i:ODH.id -> n:nonce -> h0:mem -> h1:mem -> Lemma
-////  (requires (
-////    //((modifies (Set.singleton (ODH.get_op_rgn pkae_p.op)) h0 h1 /\ (extends (ODH.get_op_rgn pkae_p.op) pkae_p.op_rgn)) \/ h0 == h1)
-////    (modifies (Set.singleton (ODH.get_op_rgn pkae_p.op)) h0 h1 \/ h0 == h1)
-////    /\ extends (ODH.get_op_rgn pkae_p.op) pkae_p.op_rgn
-////    /\ disjoint (ODH.get_op_rgn pkae_p.op) pkae_p.ap_log_rgn
-////    /\ contains h0 pkae_p.ap_log
-////    /\ (match sel h0 pkae_p.ap_log i with
-////      | Some ap -> contains h0 (AE.get_ap_log ap)
-////      | None -> True)
-////  ))
-////  (ensures (
-////    contains h1 pkae_p.ap_log
-////    /\ (match sel h0 pkae_p.ap_log i with
-////      | Some ap_old ->
-////        let ap_new = Some?.v (sel h1 pkae_p.ap_log i) in
-////        AE.get_ap_log ap_old == AE.get_ap_log ap_new
-////        /\ contains h1 (AE.get_ap_log ap_new)
-////      | None -> True)
-////    ///\ (let ap_option_new = sel h1 pkae_p.ap_log i in
-////    //ap_option_new == ap_option_old
-////    ///\ (Some? ap_option_new)
-////    ///\ AE.get_ap_log (Some?.v ap_option_new) == AE.get_ap_log (Some?.v ap_option_old))
-////  ))
-////let nonce_freshness_framing_lemma pkae_p i n h0 h1 = ()
-//
-//#set-options "--z3rlimit 300 --max_ifuel 0 --max_fuel 0"
-//val encrypt: pkae_package:pkae_package -> pk:pkey -> sk:skey{ODH.get_share_raw pk <> ODH.get_share_raw (ODH.get_exp_share sk)} -> n:nonce -> p:protected_plain pp (ODH.create_id pk (ODH.get_exp_share sk)) -> ST ciphertext
-//  (requires (fun h0 ->
-//    let i = ODH.create_id pk (ODH.get_exp_share sk) in
-//    match sel h0 pkae_package.ap_log i with
-//    | Some ap ->
-//      contains h0 (AE.get_ap_log ap)
-//      /\ AE.nonce_is_unique ap n h0
-//    | None -> True
-//  ))
-//  (ensures (fun h0 c h1 ->
-//    let i = ODH.create_id pk (ODH.get_exp_share sk) in
-//    let both_honest = ODH.exp_hon sk && ODH.sh_hon pk in
-//    let kp_log = ODH.get_op_log pkae_package.op in
-//    // Describe ap_log state
-//    Some? (sel h1 pkae_package.ap_log i)
-//    /\ (let ap = Some?.v (sel h1 pkae_package.ap_log i) in
-//    (if Some? (sel h0 pkae_package.ap_log i) then
-//      sel h1 pkae_package.ap_log == sel h0 pkae_package.ap_log
-//      /\ sel h1 (AE.get_ap_log ap) == MM.upd (sel h0 (AE.get_ap_log ap)) (n,c) p
-//    else
-//      sel h1 pkae_package.ap_log == MM.upd (sel h0 pkae_package.ap_log) i ap
-//      /\ (forall n' . n' =!= n ==> AE.nonce_is_unique ap n' h1))
-//    // Describe modified memory regions
-//    /\ (let modified_regions_ap_op = Set.union
-//        (AE.encrypt_modified_regions ap)
-//        (ODH.dh_op_modified_regions pkae_package.op pk sk h0)
-//      in
-//      let modified_regions_extend_ap_log = Set.union (Set.singleton pkae_package.ap_rgn) (Set.singleton pkae_package.ap_log_rgn) in
-//      let modified_regions =
-//        if Some? (sel h0 pkae_package.ap_log i) then
-//          modified_regions_ap_op
-//        else
-//          Set.union modified_regions_ap_op modified_regions_extend_ap_log
-//      in
-//      modifies modified_regions h0 h1)
-//    /\ ODH.dh_op_log_change pkae_package.op pk sk h0 h1
-//    // Describe functionality
-//    /\ (let k =
-//        if both_honest && ODH.get_flag() then
-//          Some?.v (MM.sel (sel h1 (ODH.get_op_log pkae_package.op)) i)
-//        else
-//          ODH.(odh_params.hash (odh_params.exponentiate (ODH.get_exponent_raw sk) (ODH.get_share_raw pk)))
-//      in
-//      ODH.dh_op_functional_spec pkae_package.op pk sk k h1
-//    )
-//    /\ ((both_honest /\ ODH.get_flag()) ==>
-//        (let k = Some?.v (MM.sel (sel h1 (ODH.get_op_log pkae_package.op)) i) in
-//        AE.encrypt_functional_spec ap k n c p)
-//      )
-//      // In case we have a dishonest key or we don't idealize, we can't guarantee anything.
-//    )
-//  ))
-//
-//#set-options "--z3rlimit 300 --max_ifuel 0 --max_fuel 0"
-//let encrypt pkae_package pk sk n p =
-//  let i = ODH.create_id pk (ODH.get_exp_share sk) in
-//  recall pkae_package.ap_log;
-//  let k = ODH.dh_op pkae_package.op pk sk in
-//  let h1 = get() in
-//  ODH.recall_op_log pkae_package.op;
-//  let ap =
-//    match get_ap_from_log pkae_package i with
-//    | Some ap ->
-//      ap
-//    | None ->
-//      let ap = AE.create_ae_package pkae_package.ap_rgn kp ae_params pp in
-//      MM.extend pkae_package.ap_log i ap;
-//      ap
-//  in
-//  let c = AE.encrypt ap k n p in
-//  //assert(
-//  //    let both_honest = ODH.exp_hon sk && ODH.sh_hon pk in
-//  //    (both_honest /\ ODH.get_flag()) ==>
-//  //      (let k' = Some?.v (MM.sel (sel h1 (ODH.get_op_log pkae_package.op)) i) in
-//  //      AE.encrypt_functional_spec ap k n c p
-//  //      )
-//  //    );
-//  //    admit();
-//  //assert(AE.encrypt_functional_spec ap k n c p);
-//  c
-//
-//val decrypt: pkae_package:pkae_package -> pk:pkey -> sk:skey{ODH.get_share_raw pk <> ODH.get_share_raw (ODH.get_exp_share sk)} -> n:nonce -> c:ciphertext -> ST (option (p:protected_plain pp (ODH.create_id pk (ODH.get_exp_share sk))))
-//  (requires (fun h0 ->
-//    let i = ODH.create_id pk (ODH.get_exp_share sk) in
-//    match sel h0 pkae_package.ap_log i with
-//    | Some ap ->
-//      contains h0 (AE.get_ap_log ap)
-//    | None -> True
-//  ))
-//  (ensures (fun h0 c h1 ->
-//    let i = ODH.create_id pk (ODH.get_exp_share sk) in
-//    let both_honest = ODH.exp_hon sk && ODH.sh_hon pk in
-//    let kp_log = ODH.get_op_log pkae_package.op in
-//    match sel h0 pkae_package.ap_log i with
-//    | Some ap ->
-//      ((both_honest /\ ODH.get_flag()) ==>
-//        (MM.defined kp_log i h0 ==>
-//          h0 == h1)
-//        /\ (MM.fresh kp_log i h0 ==>
-//          modifies (Set.singleton (ODH.get_op_rgn pkae_package.op)) h0 h1))
-//      /\ ((~both_honest \/ ~(ODH.get_flag())) ==>
-//          h0 == h1)
-//    | None ->
-//      MM.defined pkae_package.ap_log i h1
-//      /\ (let ap = Some?.v (sel h1 pkae_package.ap_log i) in
-//        sel h1 pkae_package.ap_log == MM.upd (sel h0 pkae_package.ap_log) i ap
-//        /\ ((both_honest /\ ODH.get_flag()) ==>
-//            (MM.defined kp_log i h0 ==>
-//              modifies (Set.union (Set.singleton pkae_package.ap_rgn) (Set.singleton pkae_package.ap_log_rgn)) h0 h1)
-//            /\ (MM.fresh kp_log i h0 ==>
-//              modifies (Set.union (Set.singleton pkae_package.ap_rgn) (Set.union (Set.singleton pkae_package.ap_log_rgn) (Set.singleton (ODH.get_op_rgn pkae_package.op)))) h0 h1))
-//        /\ ((~both_honest \/ ~(ODH.get_flag())) ==>
-//            (modifies (Set.union (Set.singleton pkae_package.ap_rgn) (Set.singleton pkae_package.ap_log_rgn)) h0 h1)))
-//  ))
-//
-//let decrypt pkae_package pk sk n c =
-//  let i = ODH.create_id pk (ODH.get_exp_share sk) in
-//  recall pkae_package.ap_log;
-//  let k = ODH.dh_op pkae_package.op pk sk in
-//  let ap =
-//    match get_ap_from_log pkae_package i with
-//    | Some ap ->
-//      ap
-//    | None ->
-//      let ap = AE.create_ae_package pkae_package.ap_rgn kp ae_params pp in
-//      MM.extend pkae_package.ap_log i ap;
-//      recall pkae_package.ap_log;
-//      AE.recall_log ap;
-//      ap
-//  in
-//  AE.decrypt ap k n c
+//let nonce_freshness_framing_lemma pkae_p i n h0 h1 = ()
+
+#set-options "--z3rlimit 300 --max_ifuel 0 --max_fuel 0"
+val encrypt: pkae_package:pkae_package -> pk:pkey -> sk:skey{ODH.get_share_raw pk <> ODH.get_share_raw (ODH.get_exp_share sk)} -> n:nonce -> p:protected_plain pp (ODH.create_id pk (ODH.get_exp_share sk)) -> ST ciphertext
+  (requires (fun h0 ->
+    let i = ODH.create_id pk (ODH.get_exp_share sk) in
+    match sel h0 pkae_package.ap_log i with
+    | Some ap ->
+      contains h0 (AE.get_ap_log ap)
+      /\ AE.nonce_is_unique ap n h0
+    | None -> True
+  ))
+  (ensures (fun h0 c h1 ->
+    let i = ODH.create_id pk (ODH.get_exp_share sk) in
+    let both_honest = ODH.exp_hon sk && ODH.sh_hon pk in
+    let kp_log = ODH.get_op_log pkae_package.op in
+    // Describe ap_log state
+    Some? (sel h1 pkae_package.ap_log i)
+    /\ (let ap = Some?.v (sel h1 pkae_package.ap_log i) in
+    (if Some? (sel h0 pkae_package.ap_log i) then
+      sel h1 pkae_package.ap_log == sel h0 pkae_package.ap_log
+      /\ sel h1 (AE.get_ap_log ap) == MM.upd (sel h0 (AE.get_ap_log ap)) (n,c) p
+    else
+      sel h1 pkae_package.ap_log == MM.upd (sel h0 pkae_package.ap_log) i ap
+      /\ (forall n' . n' =!= n ==> AE.nonce_is_unique ap n' h1))
+    // Describe modified memory regions
+    /\ (let modified_regions_ap_op = Set.union
+        (AE.encrypt_modified_regions ap)
+        (ODH.dh_op_modified_regions pkae_package.op pk sk h0)
+      in
+      let modified_regions_extend_ap_log = Set.union (Set.singleton pkae_package.ap_rgn) (Set.singleton pkae_package.ap_log_rgn) in
+      let modified_regions =
+        if Some? (sel h0 pkae_package.ap_log i) then
+          modified_regions_ap_op
+        else
+          Set.union modified_regions_ap_op modified_regions_extend_ap_log
+      in
+      modifies modified_regions h0 h1)
+    /\ ODH.dh_op_log_change pkae_package.op pk sk h0 h1
+    // Describe functionality
+    /\ (let k =
+        if both_honest && ODH.get_flag() then
+          Some?.v (MM.sel (sel h1 (ODH.get_op_log pkae_package.op)) i)
+        else
+          ODH.(odh_params.hash (odh_params.exponentiate (ODH.get_exponent_raw sk) (ODH.get_share_raw pk)))
+      in
+      ODH.dh_op_functional_spec pkae_package.op pk sk k h1
+    )
+    /\ ((both_honest /\ ODH.get_flag()) ==>
+        (let k = Some?.v (MM.sel (sel h1 (ODH.get_op_log pkae_package.op)) i) in
+        AE.encrypt_functional_spec ap k n c p)
+      )
+      // In case we have a dishonest key or we don't idealize, we can't guarantee anything.
+    )
+  ))
+
+#set-options "--z3rlimit 300 --max_ifuel 0 --max_fuel 0"
+let encrypt pkae_package pk sk n p =
+  let i = ODH.create_id pk (ODH.get_exp_share sk) in
+  recall pkae_package.ap_log;
+  let k = ODH.dh_op pkae_package.op pk sk in
+  let h1 = get() in
+  ODH.recall_op_log pkae_package.op;
+  let ap =
+    match get_ap_from_log pkae_package i with
+    | Some ap ->
+      ap
+    | None ->
+      let ap = AE.create_ae_package pkae_package.ap_rgn kp ae_params pp in
+      MM.extend pkae_package.ap_log i ap;
+      ap
+  in
+  let c = AE.encrypt ap k n p in
+  //assert(
+  //    let both_honest = ODH.exp_hon sk && ODH.sh_hon pk in
+  //    (both_honest /\ ODH.get_flag()) ==>
+  //      (let k' = Some?.v (MM.sel (sel h1 (ODH.get_op_log pkae_package.op)) i) in
+  //      AE.encrypt_functional_spec ap k n c p
+  //      )
+  //    );
+  //    admit();
+  //assert(AE.encrypt_functional_spec ap k n c p);
+  c
+
+val decrypt: pkae_package:pkae_package -> pk:pkey -> sk:skey{ODH.get_share_raw pk <> ODH.get_share_raw (ODH.get_exp_share sk)} -> n:nonce -> c:ciphertext -> ST (option (p:protected_plain pp (ODH.create_id pk (ODH.get_exp_share sk))))
+  (requires (fun h0 ->
+    let i = ODH.create_id pk (ODH.get_exp_share sk) in
+    match sel h0 pkae_package.ap_log i with
+    | Some ap ->
+      contains h0 (AE.get_ap_log ap)
+    | None -> True
+  ))
+  (ensures (fun h0 c h1 ->
+    let i = ODH.create_id pk (ODH.get_exp_share sk) in
+    let both_honest = ODH.exp_hon sk && ODH.sh_hon pk in
+    let kp_log = ODH.get_op_log pkae_package.op in
+    match sel h0 pkae_package.ap_log i with
+    | Some ap ->
+      ((both_honest /\ ODH.get_flag()) ==>
+        (MM.defined kp_log i h0 ==>
+          h0 == h1)
+        /\ (MM.fresh kp_log i h0 ==>
+          modifies (Set.singleton (ODH.get_op_rgn pkae_package.op)) h0 h1))
+      /\ ((~both_honest \/ ~(ODH.get_flag())) ==>
+          h0 == h1)
+    | None ->
+      MM.defined pkae_package.ap_log i h1
+      /\ (let ap = Some?.v (sel h1 pkae_package.ap_log i) in
+        sel h1 pkae_package.ap_log == MM.upd (sel h0 pkae_package.ap_log) i ap
+        /\ ((both_honest /\ ODH.get_flag()) ==>
+            (MM.defined kp_log i h0 ==>
+              modifies (Set.union (Set.singleton pkae_package.ap_rgn) (Set.singleton pkae_package.ap_log_rgn)) h0 h1)
+            /\ (MM.fresh kp_log i h0 ==>
+              modifies (Set.union (Set.singleton pkae_package.ap_rgn) (Set.union (Set.singleton pkae_package.ap_log_rgn) (Set.singleton (ODH.get_op_rgn pkae_package.op)))) h0 h1))
+        /\ ((~both_honest \/ ~(ODH.get_flag())) ==>
+            (modifies (Set.union (Set.singleton pkae_package.ap_rgn) (Set.singleton pkae_package.ap_log_rgn)) h0 h1)))
+  ))
+
+let decrypt pkae_package pk sk n c =
+  let i = ODH.create_id pk (ODH.get_exp_share sk) in
+  recall pkae_package.ap_log;
+  let k = ODH.dh_op pkae_package.op pk sk in
+  let ap =
+    match get_ap_from_log pkae_package i with
+    | Some ap ->
+      ap
+    | None ->
+      let ap = AE.create_ae_package pkae_package.ap_rgn kp ae_params pp in
+      MM.extend pkae_package.ap_log i ap;
+      recall pkae_package.ap_log;
+      AE.recall_log ap;
+      ap
+  in
+  AE.decrypt ap k n c
