secure_api/box/Box.PKAE.fsti
@@ -15,126 +15,120 @@ module MM = FStar.Monotonic.Map
 let n32 = (n:nat{n<=32})
 let bytes32 = b:bytes{Seq.length b <= 32}
 
-val random_bytes: (n:n32) -> unit -> lbytes n
-
-val pkae_flag: bool
-
 #set-options "--z3rlimit 300 --max_ifuel 1 --max_fuel 1"
 
-val valid_length: nat -> bool
-
-val pp : (pp:plain_package{pp.flag == b2t pkae_flag})
+val pp : (pp:plain_package{pp.flag == Flags.pkae})
 
 // Footpring function instead of rgn in the type
-val pkae_package: rgn:erid -> Type
+val pkae_package: rgn:erid -> Type u#1
 
-val create_pkae_package: rgn:erid -> ST (pkae_package rgn)
-  (requires (fun h0 -> True))
-  (ensures (fun h0 pkae_p h1 ->
-    modifies (Set.singleton rgn) h0 h1
-  ))
-
-//val pkey_length: n32
-let pkey_length = 32
-val pkey : Type
-val get_pkey_raw: pkey -> Tot (lbytes pkey_length)
-val get_pkey_id: pk:pkey -> Tot (i:pk_id{i = PK_id (get_pkey_raw pk)})
-
-//val skey_length: n32
-let skey_length = 32
-val skey : Type
-val get_skey_raw: skey -> GTot (lbytes pkey_length)
-val get_pkey_from_skey: skey -> pkey
-val get_skey_id: sk:skey -> Tot (i:pk_id{i = PK_id (get_pkey_raw (get_pkey_from_skey sk))})
-
-val gen : #rgn:erid -> ip:index_package rgn -> ST (keypair:(pkey*skey))
-  (requires (fun h0 -> True))
-  (ensures (fun h0 keypair h1 ->
-    get_pkey_from_skey (snd keypair) == fst keypair
-    /\ honest ip (PK_id (get_pkey_raw (fst keypair)))
-    /\ modifies (Set.singleton rgn) h0 h1
-  ))
-
-val coerce : #rgn:erid -> ip:index_package rgn -> pk_raw:lbytes pkey_length -> sk_raw:lbytes skey_length ->ST (keypair:(pkey*skey))
-  (requires (fun h0 ->
-    fresh ip (PK_id pk_raw) h0
-  ))
-  (ensures (fun h0 keypair h1 ->
-    get_pkey_from_skey (snd keypair) == fst keypair
-    /\ dishonest ip (get_pkey_id (fst keypair))
-    /\ get_pkey_raw (fst keypair) = pk_raw
-    /\ get_skey_raw (snd keypair) = sk_raw
-    /\ modifies (Set.singleton rgn) h0 h1
-  ))
-
-val compose_ids: pk_id -> pk_id -> inst_id
-
-val nonce_length:n32
-let nonce = lbytes nonce_length
-val valid_ciphertext_length : n32 -> bool
-let ciphertext = b:bytes32{valid_ciphertext_length (Seq.length b)}
-
-val compatible_keys: pkey -> skey -> bool
-
-type message_log_key =
-  | LOG_KEY: i:inst_id -> n:nonce -> c:ciphertext -> message_log_key
-
-let message_log_value (i:inst_id) = protected_plain pp i
-let message_log_range (k:message_log_key) = message_log_value (k.i)
-let message_log_inv (f:MM.map' (message_log_key) (message_log_range)) = True
-
-let message_log (rgn:erid) =
-  MM.t rgn (message_log_key) (message_log_range) (message_log_inv)
-
-val get_log: #rgn:erid -> pkae_package rgn -> message_log rgn
-
-let nonce_is_unique (#rgn:erid) (pkae_p:pkae_package rgn) (i:inst_id) (n:nonce) (h0:mem) =
-  forall c . MM.fresh (get_log pkae_p) (LOG_KEY i n c) h0
-
-let extended_message_log (#rgn:erid) (pkae_p:pkae_package rgn) (i:inst_id) (n:nonce) (c:ciphertext) (p:protected_plain pp i) (h0:mem) (h1:mem) =
-  let log_key = LOG_KEY i n c in
-  let log_value = p in
-  let log = get_log pkae_p in
-  sel h1 log == MM.upd (sel h0 log) log_key log_value
-  /\ witnessed (MM.defined log log_key)
-  /\ witnessed (MM.contains log log_key log_value)
-
-
-val enc_spec: p:plain pp -> pk:lbytes pkey_length -> sk:lbytes skey_length -> n:nonce -> c:ciphertext
-val enc_star: plain_length:n32 -> pk:lbytes pkey_length -> sk:lbytes skey_length -> n:nonce -> c:ciphertext
-val dec_spec: c:ciphertext -> pk:lbytes pkey_length -> sk:lbytes skey_length -> n:nonce -> option (p:plain pp)
-
-#set-options "--z3rlimit 300 --max_ifuel 0 --max_fuel 0"
-val encrypt: #rgn:erid -> pkae_p:pkae_package rgn -> ip:index_package rgn -> pk:pkey -> sk:skey{compatible_keys pk sk} -> n:nonce -> p:protected_plain pp (compose_ids (get_pkey_id pk) (get_skey_id sk)) -> ST ciphertext
-  (requires (fun h0 ->
-    let i = compose_ids (get_pkey_id pk) (get_skey_id sk) in
-    nonce_is_unique pkae_p i n h0
-  ))
-  (ensures (fun h0 c h1 ->
-    let i = compose_ids (get_pkey_id pk) (get_skey_id sk) in
-    //let both_honest = honest ip i in
-    modifies (Set.singleton rgn) h0 h1
-    /\ ((honest ip i /\ pkae_flag) ==>
-      c == enc_star (length p) (get_pkey_raw pk) (get_skey_raw sk) n)
-    /\ ((dishonest ip i \/ ~(b2t pkae_flag)) ==>
-      c == enc_spec (repr #rgn #pp #ip #i p) (get_pkey_raw pk) (get_skey_raw sk) n)
-    /\ extended_message_log pkae_p i n c p h0 h1
-  ))
-
-val decrypt: #rgn:erid -> pkae_p:pkae_package rgn -> ip:index_package rgn -> pk:pkey -> sk:skey{compatible_keys pk sk} -> n:nonce -> c:ciphertext -> ST (option_p:option (protected_plain pp (compose_ids (get_pkey_id pk) (get_skey_id sk))))
-  (requires (fun h0 ->
-    True
-  ))
-  (ensures (fun h0 option_p h1 ->
-    let i = compose_ids (get_pkey_id pk) (get_skey_id sk) in
-    let option_spec = dec_spec c (get_pkey_raw pk) (get_skey_raw sk) n in
-    (modifies (Set.singleton rgn) h0 h1 \/ h0 == h1)
-    /\ ((honest ip i /\ pkae_flag) ==>
-      (MM.sel (sel h0 (get_log pkae_p)) (LOG_KEY i n c) == option_p)
-      )
-    /\ ((dishonest ip i \/ ~(b2t pkae_flag)) ==>
-      (Some? option_spec ==>
-      (Some? option_p
-      /\ repr #rgn #pp #ip #i (Some?.v option_p) == Some?.v option_spec))
-      )
-  ))
+//val create_pkae_package: rgn:erid -> ST (pkae_package rgn)
+//  (requires (fun h0 -> True))
+//  (ensures (fun h0 pkae_p h1 ->
+//    modifies (Set.singleton rgn) h0 h1
+//  ))
+//
+////val pkey_length: n32
+//let pkey_length = 32
+//val pkey : Type
+//val get_pkey_raw: pkey -> Tot (lbytes pkey_length)
+//val get_pkey_id: pk:pkey -> Tot (i:pk_id{i = PK_id (get_pkey_raw pk)})
+//
+////val skey_length: n32
+//let skey_length = 32
+//val skey : Type
+//val get_skey_raw: skey -> GTot (lbytes pkey_length)
+//val get_pkey_from_skey: skey -> pkey
+//val get_skey_id: sk:skey -> Tot (i:pk_id{i = PK_id (get_pkey_raw (get_pkey_from_skey sk))})
+//
+//val gen : #rgn:erid -> ip:index_package rgn -> ST (keypair:(pkey*skey))
+//  (requires (fun h0 -> True))
+//  (ensures (fun h0 keypair h1 ->
+//    get_pkey_from_skey (snd keypair) == fst keypair
+//    /\ honest ip (PK_id (get_pkey_raw (fst keypair)))
+//    /\ modifies (Set.singleton rgn) h0 h1
+//  ))
+//
+//val coerce : #rgn:erid -> ip:index_package rgn -> pk_raw:lbytes pkey_length -> sk_raw:lbytes skey_length ->ST (keypair:(pkey*skey))
+//  (requires (fun h0 ->
+//    fresh ip (PK_id pk_raw) h0
+//  ))
+//  (ensures (fun h0 keypair h1 ->
+//    get_pkey_from_skey (snd keypair) == fst keypair
+//    /\ dishonest ip (get_pkey_id (fst keypair))
+//    /\ get_pkey_raw (fst keypair) = pk_raw
+//    /\ get_skey_raw (snd keypair) = sk_raw
+//    /\ modifies (Set.singleton rgn) h0 h1
+//  ))
+//
+//val compose_ids: pk_id -> pk_id -> inst_id
+//
+//val nonce_length:n32
+//let nonce = lbytes nonce_length
+//val valid_ciphertext_length : n32 -> bool
+//let ciphertext = b:bytes32{valid_ciphertext_length (Seq.length b)}
+//
+//val compatible_keys: pkey -> skey -> bool
+//
+//type message_log_key =
+//  | LOG_KEY: i:inst_id -> n:nonce -> c:ciphertext -> message_log_key
+//
+//let message_log_value (i:inst_id) = protected_plain pp i
+//let message_log_range (k:message_log_key) = message_log_value (k.i)
+//let message_log_inv (f:MM.map' (message_log_key) (message_log_range)) = True
+//
+//let message_log (rgn:erid) =
+//  MM.t rgn (message_log_key) (message_log_range) (message_log_inv)
+//
+//val get_log: #rgn:erid -> pkae_package rgn -> message_log rgn
+//
+//let nonce_is_unique (#rgn:erid) (pkae_p:pkae_package rgn) (i:inst_id) (n:nonce) (h0:mem) =
+//  forall c . MM.fresh (get_log pkae_p) (LOG_KEY i n c) h0
+//
+//let extended_message_log (#rgn:erid) (pkae_p:pkae_package rgn) (i:inst_id) (n:nonce) (c:ciphertext) (p:protected_plain pp i) (h0:mem) (h1:mem) =
+//  let log_key = LOG_KEY i n c in
+//  let log_value = p in
+//  let log = get_log pkae_p in
+//  sel h1 log == MM.upd (sel h0 log) log_key log_value
+//  /\ witnessed (MM.defined log log_key)
+//  /\ witnessed (MM.contains log log_key log_value)
+//
+//
+//val enc_spec: p:plain pp -> pk:lbytes pkey_length -> sk:lbytes skey_length -> n:nonce -> c:ciphertext
+////val enc_star: plain_length:n32 -> pk:lbytes pkey_length -> sk:lbytes skey_length -> n:nonce -> c:ciphertext
+//val dec_spec: c:ciphertext -> pk:lbytes pkey_length -> sk:lbytes skey_length -> n:nonce -> option (p:plain pp)
+//
+//#set-options "--z3rlimit 300 --max_ifuel 0 --max_fuel 0"
+//val encrypt: #rgn:erid -> pkae_p:pkae_package rgn -> ip:index_package rgn -> pk:pkey -> sk:skey{compatible_keys pk sk} -> n:nonce -> p:protected_plain pp (compose_ids (get_pkey_id pk) (get_skey_id sk)) -> ST ciphertext
+//  (requires (fun h0 ->
+//    let i = compose_ids (get_pkey_id pk) (get_skey_id sk) in
+//    nonce_is_unique pkae_p i n h0
+//  ))
+//  (ensures (fun h0 c h1 ->
+//    let i = compose_ids (get_pkey_id pk) (get_skey_id sk) in
+//    //let both_honest = honest ip i in
+//    modifies (Set.singleton rgn) h0 h1
+//    /\ ((honest ip i /\ Flags.pkae) ==>
+//      c == enc_star (length p) (get_pkey_raw pk) (get_skey_raw sk) n)
+//    /\ ((dishonest ip i \/ ~(Flags.pkae)) ==>
+//      c == enc_spec (repr #rgn #pp #ip #i p) (get_pkey_raw pk) (get_skey_raw sk) n)
+//    /\ extended_message_log pkae_p i n c p h0 h1
+//  ))
+//
+//val decrypt: #rgn:erid -> pkae_p:pkae_package rgn -> ip:index_package rgn -> pk:pkey -> sk:skey{compatible_keys pk sk} -> n:nonce -> c:ciphertext -> ST (option_p:option (protected_plain pp (compose_ids (get_pkey_id pk) (get_skey_id sk))))
+//  (requires (fun h0 ->
+//    True
+//  ))
+//  (ensures (fun h0 option_p h1 ->
+//    let i = compose_ids (get_pkey_id pk) (get_skey_id sk) in
+//    let option_spec = dec_spec c (get_pkey_raw pk) (get_skey_raw sk) n in
+//    (modifies (Set.singleton rgn) h0 h1 \/ h0 == h1)
+//    /\ ((honest ip i /\ Flags.pkae) ==>
+//      (MM.sel (sel h0 (get_log pkae_p)) (LOG_KEY i n c) == option_p)
+//      )
+//    /\ ((dishonest ip i \/ ~(Flags.pkae)) ==>
+//      (Some? option_spec ==>
+//      (Some? option_p
+//      /\ repr #rgn #pp #ip #i (Some?.v option_p) == Some?.v option_spec))
+//      )
+//  ))
